***NO_CI*** using sel_tot and upd_tot to define read and write for mrefs

ulib/FStar.MRef.MST2.fst
@@ -2,7 +2,7 @@ module FStar.MRef.MST2
 
 open FStar.Monotonic.Heap
 
-module MH = FStar.Monotonic.Heap
+(* TODO: Use the module system to properly control the visibility of actions and functions *)
 
 (* Preordered relations and stable predicates *)
 
@@ -17,7 +17,7 @@ let preorder (a:Type) = rel:relation a{preorder_rel rel}
 
 let stable_rel (#a:Type) (rel:relation a{preorder_rel rel}) (p:predicate a) =
   forall x y . p x /\ rel x y ==> p y
-  
+
 
 (* Defining the underlying state monad on mem using DM4F *)
 
@@ -28,7 +28,6 @@ let return_st (a:Type) (x:a) : st a = fun h0 -> x, h0
 let bind_st (a:Type) (b:Type) (f:st a) (g:a -> st b) : st b
   = fun (h0:heap) -> let (x,h) = f h0 in g x h
 
-(* Actions *)
 let get_st () : st heap = fun h0 -> h0, h0
 
 let put_st (x:heap) : st unit = fun _ -> (), x
@@ -38,103 +37,78 @@ total new_effect {
   with repr     = st
      ; bind     = bind_st
      ; return   = return_st
-     ; get      = get_st
-     ; put      = put_st
+     ; get_st      = get_st
+     ; put_st      = put_st
 }
 
-//let reln (a:Type) = a -> a -> Type
 
-//let monotonic (a:Type) (b:reln a) =
-//  (forall x. b x x)                             (* reflexive *)
-//  /\ (forall x y z. b x y /\ b y z ==> b x z)   (* transitive *)
+(* Pre- and postcondition form of MSTATE *)
 
-abstract let mref (a:Type) (rel:preorder a) = MH.mref a rel
+let st_pre = heap -> Type0
+let st_post a = a -> heap -> Type0
 
-val as_mref: #a:Type -> #rel:preorder a -> mref a rel -> GTot (mref a rel)
-let as_mref #a #rel m = m
+effect MST (a:Type) (pre:st_pre) (post: (heap -> Tot (st_post a))) =
+       MSTATE a
+             (fun (h0:heap) (p:(a * heap) -> Type0) -> pre h0 /\ (forall a h1. post h0 a h1 ==> p (a, h1)))
 
-let contains (#a:Type) (#rel:preorder a) (h:heap) (m:mref a rel) = MH.contains h (as_mref m)
 
-val sel: #a:Type -> #rel:preorder a -> h:heap -> mref a rel -> GTot a
-let sel #a #rel h m = MH.sel h (as_mref m)
+(* Private definition of monotonic references, used to state heap_rel *)
 
-val upd: #a:Type -> #rel:preorder a -> h:heap -> (m:mref a rel) -> (x:a{upd_condition h m x}) -> GTot heap
-let upd #a #rel h m v = MH.upd h (as_mref m) v
+private abstract let mmref (a:Type) (rel:preorder a) = mref a rel
+
+let m_as_mref (#a:Type) (#rel:preorder a) (m:mmref a rel) :GTot (mref a rel) = m
+
+let m_contains (#a:Type) (#rel:preorder a) (h:heap) (m:mmref a rel) = contains h (m_as_mref m)
+
+let m_addr_of (#a:Type) (#rel:preorder a) (m:mmref a rel) :GTot nat = addr_of (m_as_mref m)
+
+let m_sel (#a:Type) (#rel:preorder a) (h:heap) (m:mmref a rel) :GTot a 
+  = sel h (m_as_mref m)
+
+let m_upd (#a:Type) (#rel:preorder a) (h:heap) (m:mmref a rel) (x:a{upd_condition h (m_as_mref m) x}) :GTot heap 
+  = upd h (m_as_mref m) x
 
 
 (* Generated preorder on heaps *)
 
 let heap_rel (h0:heap) (h1:heap) 
-  = (forall a rel (m:mref a rel) . (contains h0 m ==> contains h1 m) )
- /\ (forall a rel (m:mref a rel) . (contains h0 m ==> rel (sel h0 m) (sel h1 m)))
+  = (forall a rel (m:mmref a rel) . (m_contains h0 m ==> m_contains h1 m) )
+ /\ (forall a rel (m:mmref a rel) . (m_contains h0 m ==> rel (m_sel h0 m) (m_sel h1 m)))
 
-(*val lemma1: (a:Type)
-         -> (rel:preorder a)
-         -> (h:heap)
-         -> (m:mref a rel)
-         -> (x:a)
-	 -> Lemma (requires (contains h m /\ rel (sel h m) x))
-	          (ensures  (rel (sel h m) x /\ (forall b rel' (m':mref b rel') . contains h m' ==> contains (upd h m x) m')))
-let lemma1 a rel h m x = ()
 
-val lemma2: (a:Type)
-         -> (rel:preorder a)
-         -> (h:heap)
-         -> (m:mref a rel)
-         -> (x:a)
-	 -> Lemma (requires (contains h m /\ rel (sel h m) x))
-	          (ensures  (rel (sel h m) x /\ (forall b rel' (m':mref b rel') . addr_of m <> addr_of m' /\ contains h m' ==> rel' (sel h m') (sel (upd h m x) m'))))
-let lemma2 a rel h m x = ()
+(* Lifting a relation on reference to heap_rel *)
 
-val lemma3: (a:Type)
-         -> (rel:preorder a)
-         -> (h:heap)
-         -> (m:mref a rel)
-         -> (x:a)
-	 -> Lemma (requires (contains h m /\ rel (sel h m) x))
-	          (ensures  (rel (sel h m) x /\ sel (upd h m x) m == x))
-let lemma3 a rel h m x = ()*)
+val m_lifting_lemma_aux: (#a:Type)
+	              -> (#b:Type)
+                      -> (#rel:preorder a)
+	              -> (#rel':preorder b)
+                      -> (h:heap)
+                      -> (m:mmref a rel)
+	              -> (m':mmref b rel')
+                      -> (x:a)
+	              -> Lemma (requires (m_contains h m /\ rel (m_sel h m) x /\ m_addr_of m = m_addr_of m' /\ m_contains h m'))
+	                       (ensures  (rel (m_sel h m) x /\ rel' (m_sel h m') (m_sel (m_upd h m x) m')))
+		               [SMTPat (m_contains h m'); SMTPat (rel (m_sel h m) x)]
+let m_lifting_lemma_aux #a #b #rel #rel' h m m' x = lemma_contains_same_type h (m_as_mref m) (m_as_mref m'); lemma_contains_same_rel h (m_as_mref m) (m_as_mref m')
 
-val lifting_lemma_aux: (#a:Type)
-	            -> (#b:Type)
-                    -> (#rel:preorder a)
-	            -> (#rel':preorder b)
-                    -> (h:heap)
-                    -> (m:mref a rel)
-	            -> (m':mref b rel')
-                    -> (x:a)
-	            -> Lemma (requires (contains h m /\ rel (sel h m) x /\ addr_of m = addr_of m' /\ contains h m'))
-	                     (ensures  (contains h m /\ rel (sel h m) x /\ rel' (sel h m') (sel (upd h m x) m')))
-		             [SMTPat (contains h m'); SMTPat (rel (sel h m) x)]
-let lifting_lemma_aux #a #b #rel #rel' h m m' x = lemma_contains_same_type h m m'; lemma_contains_same_rel h m m'; ()
-
-(*val lemma5: (a:Type)
-         -> (rel:preorder a)
-         -> (h:heap)
-         -> (m:mref a rel)
-         -> (x:a)
-	 -> Lemma (requires (contains h m /\ rel (sel h m) x))
-	          (ensures  (contains h m /\ rel (sel h m) x /\ (forall b rel' (m':mref b rel') . addr_of m = addr_of m' /\ contains h m' ==> rel' (sel h m') (sel (upd h m x) m'))))
-let lemma5 a rel h m x = ()*)
-
-val lifting_lemma: (#a:Type) 
-                -> (#rel:preorder a) 
-	        -> (h:heap)
-	        -> (m:mref a rel) 
-	        -> (x:a)
-	        -> Lemma (requires (contains h m /\ rel (sel h m) x))
-		         (ensures  (contains h m /\ rel (sel h m) x /\ heap_rel h (upd h m x)))
-			 [SMTPat (heap_rel h (upd h m x))]
-let lifting_lemma #a #rel h m x = ()
+val m_lifting_lemma: (#a:Type) 
+                  -> (#rel:preorder a) 
+	          -> (h:heap)
+	          -> (m:mmref a rel) 
+	          -> (x:a)
+	          -> Lemma (requires (m_contains h m /\ rel (m_sel h m) x))
+		           (ensures  (m_contains h m /\ rel (m_sel h m) x /\ heap_rel h (m_upd h m x)))
+			   [SMTPat (heap_rel h (m_upd h m x))]
+let m_lifting_lemma #a #rel h m x = ()
 
 
 (* The preorder-indexed monad interface for MSTATE *)
 
 val mst_get: unit -> MST heap (fun _ -> True) (fun h0 h h1 -> h0 == h /\ h == h1)
-let mst_get () = MSTATE?.get ()
+let mst_get () = MSTATE?.get_st ()
 
 val mst_put: h:heap -> MST unit (fun h0 -> heap_rel h0 h) (fun _ _ h1 -> h == h1)
-let mst_put h = MSTATE?.put h
+let mst_put h = MSTATE?.put_st h
 
 abstract type mst_witnessed (p:predicate heap{stable heap_rel p}) = True
 
@@ -144,11 +118,65 @@ let mst_witness p = ()
 val mst_recall: p:predicate heap{stable heap_rel p} -> MST unit (fun _ -> mst_witnessed p) (fun h0 _ h1 -> h0 == h1 /\ p h1)
 let mst_recall p = admit () //intentional (justified by metatheory)
 
-let stable (#a:Type) (p:predicate a) (rel:preorder a) = stable_rel rel p
 
-abstract type token (#a:Type) (#rel:preorder a) (m:mref a rel) (p:predicate a{stable p rel}) = True
+(* Monotonic references and operations on them *)
 
-(* The monotonic references interface for MSTATE *)
+abstract let mref (a:Type) (rel:preorder a) = m:mmref a rel{mst_witnessed (fun h -> m_contains h m)}
+
+let as_mref (#a:Type) (#rel:preorder a) (m:mref a rel) :GTot (FStar.Monotonic.Heap.mref a rel) = m_as_mref m
+
+let as_mmref (#a:Type) (#rel:preorder a) (m:mref a rel) :GTot (mmref a rel) = m
+
+let contains (#a:Type) (#rel:preorder a) (h:heap) (m:mref a rel) = contains h (as_mref m)
+
+let addr_of (#a:Type) (#rel:preorder a) (m:mref a rel) :GTot nat = addr_of (as_mref m)
+
+let sel (#a:Type) (#rel:preorder a) (h:heap) (m:mref a rel) :GTot a = sel h (as_mref m)
+
+let upd (#a:Type) (#rel:preorder a) (h:heap) (m:mref a rel) (x:a{upd_condition h (as_mref m) x}) :GTot heap = upd h (as_mref m) x
+
+
+(* Lifting a relation on mref to heap_rel *)
+
+val lifting_lemma: (#a:Type) 
+                -> (#rel:preorder a) 
+	        -> (h:heap)
+	        -> (m:mref a rel) 
+	        -> (x:a)
+	        -> Lemma (requires (contains h m /\ rel (sel h m) x))
+		         (ensures  (contains h m /\ rel (sel h m) x /\ heap_rel h (upd h m x)))
+			 [SMTPat (heap_rel h (upd h m x))]
+let lifting_lemma #a #rel h m x = m_lifting_lemma h (as_mmref m) x
+
+
+(* The public monotonic references interface for MSTATE *)
+
+val read: #a:Type
+       -> #rel:preorder a
+       -> m:mref a rel
+       -> MST a
+              (requires (fun h -> True))
+              (ensures  (fun h0 v h1 -> h0 == h1 /\ v == sel h0 m))
+let read #a #rel m 
+  = let h = mst_get () in
+    mst_recall (fun h -> contains h m);
+    FStar.Monotonic.Heap.sel_tot h m
+    
+
+val write: #a:Type
+        -> #rel:preorder a
+        -> m:mref a rel
+        -> x:a
+        -> MST unit
+               (requires (fun h0 -> rel (sel h0 m) x))
+               (ensures  (fun h0 _ h1 -> rel (sel h0 m) x /\ h1 == upd h0 m x))
+let write #a #rel m x 
+  = let h0 = mst_get () in
+    mst_recall (fun h -> contains h m);
+    let h1 = FStar.Monotonic.Heap.upd_tot h0 m x in
+    assert (h1 == upd h0 m x);
+    mst_put h1
+
 
 (*type fresh(#a:Type) (#rel:preorder a) (x:a) h0 (m:mref a rel) h1 = 
   ~ (contains h0 m) /\ contains h1 m /\ h1 == upd h0 m x
@@ -161,22 +189,13 @@ val alloc: #a:Type
               (fun h0 m h1 -> fresh x h0 m h1)
 let alloc #a #rel x 
   = let h0 = mst_get () in
-    let mh = alloc h0 x rel false in 
+    //let mh = alloc h0 x rel false in 
     admit () //ST.alloc x*)
-
-(*val read: #a:Type
-       -> #rel:preorder a
-       -> m:mref a rel
-       -> MST a
-              (requires (fun h -> True))
-              (ensures  (fun h0 v h1 -> h0 == h1 /\ v == sel h0 m))
-let read #a #b m = 
-  let h = mst_get () in
-  sel h m*)
-
 
 
 (*
+
+let stable (#a:Type) (p:predicate a) (rel:preorder a) = stable_rel rel p
 
 abstract type token (#a:Type) (#rel:preorder a) (m:mref a rel) (p:predicate a{stable p rel}) = True
 abstract type witnessed (p:heap -> Type) = True
@@ -242,3 +261,5 @@ val witness: #a:Type
                 (requires (fun h0 -> p h0 /\ stable_on_heap m p))
                 (ensures (fun h0 _ h1 -> h0==h1 /\ witnessed p))
 let witness #a #b m p = ()*)
+
+
